\chapter{Signals \& Systems}

\section{Fourier Series}

Cosine/Sine Representation
\begin{align*}
&f(t) = a_0 + \sum_{n=1}^{\infty}\left[a_n \cos(2\pi nf_0 t) + b_n \sin(2\pi nf_0 t)\right],\; f_0 = \frac{1}{T}\\
&a_0 = \frac{1}{T}\int_{0}^{T}f(t)dt, \qquad a_n = \frac{2}{T}\int_{0}^{T}f(t)\cos(2\pi nf_0 t)dt,\\
&b_n = \frac{2}{T}\int_{0}^{T} f(t)\sin(2\pi nf_0 t)dt\\
\end{align*}
Amplitude/Phase Representation
\begin{align*}
&f(t) = a_0 + \sum_{n=1}^{\infty}c_n \cos(2\pi nf_0 + \phi_n),\; f_0 = \frac{1}{T}\\
&a_0 = \frac{1}{T}\int_{0}^{T}f(t)dt, \quad c_n = \sqrt{a_n^2 + b_n^2}\\
&\phi_n = \begin{cases}
-\arctan(b_n / a_n) & a_n > 0\\
\pi -\arctan(b_n / a_n) & a_n < 0\\
\end{cases}
\end{align*}
Exponential Representation
\begin{gather*}
f(t)=\sum_{n=-\infty}^{\infty}\mathbf{x}_n e^{jn\omega_0 t}\\
\mathbf{x}_n=\left|\mathbf{x}_n\right|e^{j\phi_n}, \quad \mathbf{x}_{-n}=\mathbf{x}_n^*, \quad \phi_{-n}=-\phi_n, \quad \left|\mathbf{x}_n\right|=c_n/2, \quad x_0=c_0 \\
\mathbf{x}_n=\frac{1}{T_0}\int_{0}^{T_0}x(t)e^{-jn\omega_0 t}dt
\end{gather*}



%\begin{mybox}{Fourier Series}
%	Cosine/Sine Representation
%	\begin{align*}
%	&f(t) = a_0 + \sum_{n=1}^{\infty}\left[a_n \cos(2\pi nf_0 t) + b_n \sin(2\pi nf_0 t)\right],\; f_0 = \frac{1}{T}\\
%	&a_0 = \frac{1}{T}\int_{0}^{T}f(t)dt, \qquad a_n = \frac{2}{T}\int_{0}^{T}f(t)\cos(2\pi nf_0 t)dt,\\
%	&b_n = \frac{2}{T}\int_{0}^{T} f(t)\sin(2\pi nf_0 t)dt\\
%	\end{align*}
%	Amplitude/Phase Representation
%	\begin{align*}
%	&f(t) = a_0 + \sum_{n=1}^{\infty}c_n \cos(2\pi nf_0 + \phi_n),\; f_0 = \frac{1}{T}\\
%	&a_0 = \frac{1}{T}\int_{0}^{T}f(t)dt, \quad c_n = \sqrt{a_n^2 + b_n^2}\\
%	&\phi_n = \begin{cases}
%	-\arctan(b_n / a_n) & a_n > 0\\
%	\pi -\arctan(b_n / a_n) & a_n < 0\\
%	\end{cases}
%	\end{align*}
%\end{mybox}

\section{Fourier Transform}
\begin{align*}
F\left[x(t)\right] &= X(\omega) = \int_{-\infty}^{\infty}x(t)e^{-j\omega t}dt \\
x(t) &= F^{-1}\left[X(\omega)\right] = \frac{1}{2\pi}\int_{-\infty}^{\infty}X(\omega)e^{-j\omega t}d\omega
\end{align*}

\section{Convolution}
\[x(t) * h(t) = \int_{-\infty}^{\infty}x(\tau)h(t-\tau)d\tau\]

\section{Discrete Time}
Sampling concepts:
\begin{itemize}
\item $\delta T_s(t) = \sum_{-\infty}_^{\infty} \delta(t-nT_s)$
\item $\delta T_s(f) = \frac{1}{T_s}\sum_{-\infty}^{\infty} \delta(f-nf_s)
\end{itemize}


%\begin{mybox}{Fourier Transform}
%\begin{align*}
%F\left[x(t)\right] &= X(\omega) = \int_{-\infty}^{\infty}x(t)e^{-j\omega t}dt \\
%x(t) &= F^{-1}\left[X(\omega)\right] = \frac{1}{2\pi}\int_{-\infty}^{\infty}X(\omega)e^{-j\omega t}d\omega
%\end{align*}
%Hey there
%\end{mybox}

%\begin{mybox}{Convolution Integral}
%\[x(t) * h(t) = \int_{-\infty}^{\infty}x(\tau)h(t-\tau)d\tau\]
%Other stuff
%\end{mybox}
